Experiments/Test_Suite_IO.thy
@@ -1,94 +1,12 @@
+section \<open>Representing Test Suites as Sets of Input-Output Sequences\<close>
+
+text \<open>This theory describes the representation of test suites as sets of input-output sequences
+      and defines a pass relation for this representation.\<close>
+
+
 theory Test_Suite_IO
 imports Test_Suite Maximal_Path_Trie
 begin
-
-
-section \<open>Representing Test Suites as Sets of Input/Output Sequences\<close>
-
-
-lemma preamble_maximal_io_paths :
-  assumes "is_preamble P M q"
-  and     "observable M"
-  and     "path P (initial P) p"
-  and     "target (initial P) p = q"
-shows "\<nexists>io' . io' \<noteq> [] \<and> p_io p @ io' \<in> L P" 
-proof -
-  have "deadlock_state P q"  
-  and  "is_submachine P M"
-    using assms(1) unfolding is_preamble_def by blast+
-
-  have "observable P"
-    using \<open>observable M\<close> \<open>is_submachine P M\<close>
-    using submachine_observable by blast 
-
-  show "\<nexists>io' . io' \<noteq> [] \<and> p_io p @ io' \<in> L P"
-  proof
-    assume "\<exists>io'. io' \<noteq> [] \<and> p_io p @ io' \<in> L P"
-    then obtain io' where "io' \<noteq> []" and "p_io p @ io' \<in> L P"
-      by blast
-
-    obtain p1 p2 where "path P (FSM.initial P) p1" and "path P (target (FSM.initial P) p1) p2" and "p_io p1 = p_io p" and "p_io p2 = io'"
-      using language_state_split[OF \<open>p_io p @ io' \<in> L P\<close>] by blast
-
-    have "p1 = p"
-      using observable_path_unique[OF \<open>observable P\<close> \<open>path P (FSM.initial P) p1\<close> \<open>path P (FSM.initial P) p\<close> \<open>p_io p1 = p_io p\<close>] by assumption
-
-    have "io' \<in> LS P q"
-      using \<open>path P (target (FSM.initial P) p1) p2\<close> \<open>p_io p2 = io'\<close>
-      unfolding \<open>p1 = p\<close> assms(4) by auto
-    then show "False"
-      using \<open>io' \<noteq> []\<close> \<open>deadlock_state P q\<close> unfolding deadlock_state_alt_def by blast
-  qed
-qed
-
-
-
-lemma preamble_maximal_io_paths_rev :
-  assumes "is_preamble P M q"
-  and     "observable M"
-  and     "io \<in> L P"
-  and     "\<nexists>io' . io' \<noteq> [] \<and> io @ io' \<in> L P"
-obtains p where "path P (initial P) p"
-          and   "p_io p = io"
-          and   "target (initial P) p = q"
-proof -
-  
-  have "acyclic P"
-  and  "deadlock_state P q"  
-  and  "is_submachine P M"
-  and  "\<And> q' . q'\<in>reachable_nodes P \<Longrightarrow> (q = q' \<or> \<not> deadlock_state P q')"
-    using assms(1) unfolding is_preamble_def by blast+
-
-  have "observable P"
-    using \<open>observable M\<close> \<open>is_submachine P M\<close>
-    using submachine_observable by blast 
-
-  obtain p where "path P (initial P) p" and "p_io p = io"
-    using \<open>io \<in> L P\<close> by auto
-
-  moreover have "target (initial P) p = q"
-  proof (rule ccontr)
-    assume "target (FSM.initial P) p \<noteq> q"
-    then have "\<not> deadlock_state P (target (FSM.initial P) p)"
-      using \<open>\<And> q' . q'\<in>reachable_nodes P \<Longrightarrow> (q = q' \<or> \<not> deadlock_state P q')\<close>[OF reachable_nodes_intro[OF \<open>path P (initial P) p\<close>]] by simp
-    then obtain t where "t \<in> transitions P" and "t_source t = target (initial P) p"
-      by auto
-    then have "path P (initial P) (p @ [t])"
-      using path_append_transition[OF \<open>path P (initial P) p\<close>] by auto
-    then have "p_io (p@[t]) \<in> L P"
-      unfolding LS.simps by (metis (mono_tags, lifting) mem_Collect_eq)
-    then have "io @ [(t_input t, t_output t)] \<in> L P"
-      using \<open>p_io p = io\<close> by auto
-    then show "False"
-      using assms(4) by auto
-  qed
-
-  ultimately show ?thesis using that by blast
-qed
-
-
-
-
 
 
 fun test_suite_to_io :: "('a,'b,'c) fsm \<Rightarrow> ('a,'b,'c,'d) test_suite \<Rightarrow> ('b \<times> 'c) list set" where
@@ -96,9 +14,6 @@ fun test_suite_to_io :: "('a,'b,'c) fsm \<Rightarrow> ('a,'b,'c,'d) test_suite \
     (\<Union> (q,P) \<in> prs . L P)
     \<union> (\<Union>{(\<lambda> io' . p_io p @ io') ` (set (prefixes (p_io pt))) | p pt . \<exists> q P . (q,P) \<in> prs \<and> path P (initial P) p \<and> target (initial P) p = q \<and> pt \<in> tps q})
     \<union> (\<Union>{(\<lambda> io_atc . p_io p @ p_io pt @ io_atc) ` (atc_to_io_set (from_FSM M (target q pt)) A) | p pt q A . \<exists> P q' t1 t2 . (q,P) \<in> prs \<and> path P (initial P) p \<and> target (initial P) p = q \<and> pt \<in> tps q \<and> q' \<in> rd_targets (q,pt) \<and> (A,t1,t2) \<in> atcs (target q pt,q') })"
-
-
-
 
 
 lemma test_suite_to_io_language :
@@ -110,28 +25,28 @@ proof
   obtain prs tps rd_targets atcs where "T = Test_Suite prs tps rd_targets atcs"
     by (meson test_suite.exhaust)
 
-
-
   then obtain RepSets where RepSets_def: "is_sufficient_for_reduction_testing_for_RepSets (Test_Suite prs tps rd_targets atcs) M m RepSets"
-    using assms(1) unfolding is_sufficient_for_reduction_testing_def by blast
+    using assms(1) unfolding is_sufficient_for_reduction_testing_def 
+    by blast
   then have "is_sufficient_for_reduction_testing (Test_Suite prs tps rd_targets atcs) M m"
-    unfolding is_sufficient_for_reduction_testing_def by blast
-
+    unfolding is_sufficient_for_reduction_testing_def 
+    by blast
 
   have t2: "\<And> q P. (q, P) \<in> prs \<Longrightarrow> is_preamble P M q"
-    using is_sufficient_for_reduction_testing_for_RepSets_simps(2)[OF RepSets_def] by blast
+    using is_sufficient_for_reduction_testing_for_RepSets_simps(2)[OF RepSets_def] 
+    by blast
   
   have t5: "\<And>q. q \<in> FSM.nodes M \<Longrightarrow> (\<exists>d\<in>set RepSets. q \<in> fst d)"
-    using is_sufficient_for_reduction_testing_for_RepSets_simps(4)[OF RepSets_def] by assumption
+    using is_sufficient_for_reduction_testing_for_RepSets_simps(4)[OF RepSets_def] 
+    by assumption
 
   have t6: "\<And> q. q \<in> fst ` prs \<Longrightarrow> tps q \<subseteq> {p1 . \<exists> p2 d . (p1@p2,d) \<in> m_traversal_paths_with_witness M q RepSets m} \<and> fst ` (m_traversal_paths_with_witness M q RepSets m) \<subseteq> tps q"
-    using is_sufficient_for_reduction_testing_for_RepSets_simps(7)[OF RepSets_def] by assumption
+    using is_sufficient_for_reduction_testing_for_RepSets_simps(7)[OF RepSets_def] 
+    by assumption
 
   have t8: "\<And> d. d \<in> set RepSets \<Longrightarrow> snd d \<subseteq> fst d"
     using is_sufficient_for_reduction_testing_for_RepSets_simps(5,6)[OF RepSets_def] 
     by blast
-
-  
 
 
   from \<open>io \<in> test_suite_to_io M T\<close> consider
@@ -153,8 +68,12 @@ proof
       using submachine_language[OF \<open>is_submachine P M\<close>] \<open>io \<in> L P\<close> by blast
   next
     case b
-    then obtain p pt q P where "io \<in> (\<lambda> io' . p_io p @ io') ` (set (prefixes (p_io pt)))" and "(q,P) \<in> prs" and "path P (initial P) p" and "target (initial P) p = q" and "pt \<in> tps q"
-      by blast
+    then obtain p pt q P where "io \<in> (\<lambda> io' . p_io p @ io') ` (set (prefixes (p_io pt)))" 
+                           and "(q,P) \<in> prs" 
+                           and "path P (initial P) p" 
+                           and "target (initial P) p = q" 
+                           and "pt \<in> tps q"
+      by blast 
 
     then obtain io' where "io = p_io p @ io'" and "io' \<in> (set (prefixes (p_io pt)))"
       by blast
@@ -168,35 +87,44 @@ proof
         using a1 \<open>io = p_io p @ io'\<close> by moura
     qed 
 
-
-
     have "q \<in> fst ` prs"
-      using \<open>(q,P) \<in> prs\<close> by force
-
-    
+      using \<open>(q,P) \<in> prs\<close> 
+      by force
 
     have "is_submachine P M"
-      using t2[OF \<open>(q, P) \<in> prs\<close>] unfolding is_preamble_def by blast
-    then have "initial P = initial M" by auto
+      using t2[OF \<open>(q, P) \<in> prs\<close>] 
+      unfolding is_preamble_def 
+      by blast
+    then have "initial P = initial M" 
+      by auto
 
     have "path M (initial M) p"
-      using submachine_path[OF \<open>is_submachine P M\<close> \<open>path P (initial P) p\<close>] unfolding \<open>initial P = initial M\<close> by assumption
+      using submachine_path[OF \<open>is_submachine P M\<close> \<open>path P (initial P) p\<close>] 
+      unfolding \<open>initial P = initial M\<close> 
+      by assumption
+
     have "target (initial M) p = q"
-      using \<open>target (initial P) p = q\<close> unfolding \<open>initial P = initial M\<close> by assumption
+      using \<open>target (initial P) p = q\<close> 
+      unfolding \<open>initial P = initial M\<close> 
+      by assumption
 
     obtain p2 d where "(pt @ p2, d) \<in> m_traversal_paths_with_witness M q RepSets m"
-      using t6[OF \<open>q \<in> fst ` prs\<close>] \<open>pt \<in> tps q\<close> by blast
-
+      using t6[OF \<open>q \<in> fst ` prs\<close>] \<open>pt \<in> tps q\<close> 
+      by blast
     then have "path M q (pt @ p2)"
       using m_traversal_paths_with_witness_set[OF t5 t8 path_target_is_node[OF \<open>path M (initial M) p\<close>], of m]
-      unfolding \<open>target (initial M) p = q\<close> by blast
+      unfolding \<open>target (initial M) p = q\<close> 
+      by blast
     then have "path M (initial M) (p@pt)"
-      using \<open>path M (initial M) p\<close> \<open>target (initial M) p = q\<close> by auto
+      using \<open>path M (initial M) p\<close> \<open>target (initial M) p = q\<close> 
+      by auto
     then have "p_io p @ p_io pt \<in> L M"
       by (metis (mono_tags, lifting) language_intro map_append)
     
     then show "io \<in> L M"
-      unfolding \<open>io = p_io p @ io'\<close> \<open>p_io pt = io' @ io''\<close> append.assoc[symmetric] using language_prefix[of "p_io p @ io'" io'' M "initial M"] by blast
+      unfolding \<open>io = p_io p @ io'\<close> \<open>p_io pt = io' @ io''\<close> append.assoc[symmetric] 
+      using language_prefix[of "p_io p @ io'" io'' M "initial M"] 
+      by blast
   next
     case c
                                                                                                                       
@@ -226,47 +154,49 @@ proof
     then have "initial P = initial M" by auto
 
     have "path M (initial M) p"
-      using submachine_path[OF \<open>is_submachine P M\<close> \<open>path P (initial P) p\<close>] unfolding \<open>initial P = initial M\<close> by assumption
+      using submachine_path[OF \<open>is_submachine P M\<close> \<open>path P (initial P) p\<close>] 
+      unfolding \<open>initial P = initial M\<close> 
+      by assumption
     have "target (initial M) p = q"
-      using \<open>target (initial P) p = q\<close> unfolding \<open>initial P = initial M\<close> by assumption
+      using \<open>target (initial P) p = q\<close> 
+      unfolding \<open>initial P = initial M\<close> 
+      by assumption
 
     obtain p2 d where "(pt @ p2, d) \<in> m_traversal_paths_with_witness M q RepSets m"
       using t6[OF \<open>q \<in> fst ` prs\<close>] \<open>pt \<in> tps q\<close> by blast
 
     then have "path M q (pt @ p2)"
       using m_traversal_paths_with_witness_set[OF t5 t8 path_target_is_node[OF \<open>path M (initial M) p\<close>], of m]
-      unfolding \<open>target (initial M) p = q\<close> by blast
+      unfolding \<open>target (initial M) p = q\<close> 
+      by blast
     then have "path M (initial M) (p@pt)"
-      using \<open>path M (initial M) p\<close> \<open>target (initial M) p = q\<close> by auto
-
+      using \<open>path M (initial M) p\<close> \<open>target (initial M) p = q\<close> 
+      by auto
     moreover have "(target q pt) = target (initial M) (p@pt)"
-      using \<open>target (initial M) p = q\<close> by auto
-
+      using \<open>target (initial M) p = q\<close>
+      by auto
     ultimately have "(target q pt) \<in> nodes M"
-      using path_target_is_node by metis
+      using path_target_is_node 
+      by metis
 
     have "ioA \<in> LS M (target q pt)"
-      using from_FSM_language[OF \<open>(target q pt) \<in> nodes M\<close>] \<open>ioA \<in> L (from_FSM M (target q pt))\<close> by blast
+      using from_FSM_language[OF \<open>(target q pt) \<in> nodes M\<close>] \<open>ioA \<in> L (from_FSM M (target q pt))\<close>
+      by blast
     then obtain pA where "path M (target q pt) pA" and "p_io pA = ioA"
       by auto
-
     then have "path M (initial M) (p @ pt @ pA)"
-      using \<open>path M (initial M) (p@pt)\<close>  unfolding \<open>(target q pt) = target (initial M) (p@pt)\<close> by auto
+      using \<open>path M (initial M) (p@pt)\<close>  unfolding \<open>(target q pt) = target (initial M) (p@pt)\<close> 
+      by auto
     then have "p_io p @ p_io pt @ ioA \<in> L M"
       unfolding \<open>p_io pA = ioA\<close>[symmetric]
       using language_intro by fastforce
     then show "io \<in> L M"
-      unfolding \<open>io = p_io p @ p_io pt @ ioA\<close> by assumption
+      unfolding \<open>io = p_io p @ p_io pt @ ioA\<close> 
+      by assumption
   qed
 qed
 
   
-  
-
-
-
-
-
 lemma minimal_io_seq_to_failure :
   assumes "\<not> (L M' \<subseteq> L M)"
   and     "inputs M' = inputs M"  
@@ -294,12 +224,14 @@ proof -
   then have "butlast ioF' \<notin> ?prefs"
     using \<open>\<And> ioF'' . ioF'' \<in> ?prefs \<Longrightarrow> length ioF' \<le> length ioF''\<close> leD by blast 
   moreover have "butlast ioF' \<in> L M'"
-    using \<open>ioF' \<in> L M'\<close> language_prefix[of "butlast ioF'" "[last ioF']" M' "initial M'"] unfolding \<open>ioF' = (butlast ioF')@[last ioF']\<close>[symmetric] by blast
+    using \<open>ioF' \<in> L M'\<close> language_prefix[of "butlast ioF'" "[last ioF']" M' "initial M'"] 
+    unfolding \<open>ioF' = (butlast ioF')@[last ioF']\<close>[symmetric] by blast
   moreover have "butlast ioF' \<in> set (prefixes ioF)"
     using \<open>ioF' = (butlast ioF')@[last ioF']\<close> \<open>ioF' \<in> ?prefs\<close> prefixes_set
   proof -
     have "\<exists>ps. (butlast ioF' @ [last ioF']) @ ps = ioF"
-      using \<open>ioF' = butlast ioF' @ [last ioF']\<close> \<open>ioF' \<in> {ioF' \<in> set (prefixes ioF). ioF' \<in> L M' \<and> ioF' \<notin> L M}\<close> prefixes_set by auto
+      using \<open>ioF' = butlast ioF' @ [last ioF']\<close> \<open>ioF' \<in> {ioF' \<in> set (prefixes ioF). ioF' \<in> L M' \<and> ioF' \<notin> L M}\<close> prefixes_set 
+      by auto
     then show ?thesis
       using prefixes_set by fastforce
   qed
@@ -313,43 +245,31 @@ proof -
   
   obtain p where "path M (initial M) p" and "p_io p = butlast ioF'"
     using \<open>butlast ioF' \<in> L M\<close> by auto
-  moreover obtain t where "t \<in> transitions M" and "t_source t = target (initial M) p" and "t_input t = fst (last ioF')"
+  moreover obtain t where "t \<in> transitions M" 
+                      and "t_source t = target (initial M) p" 
+                      and "t_input t = fst (last ioF')"
   proof -
     have "fst (last ioF') \<in> inputs M'"
-      using language_io(1)[OF *, of "fst (last ioF')" "snd (last ioF')"] by simp 
+      using language_io(1)[OF *, of "fst (last ioF')" "snd (last ioF')"] 
+      by simp 
     then have "fst (last ioF') \<in> inputs M"
       using assms(2) by auto
     then show ?thesis
-      using that \<open>completely_specified M\<close> path_target_is_node[OF \<open>path M (initial M) p\<close>] unfolding completely_specified.simps by blast
+      using that \<open>completely_specified M\<close> path_target_is_node[OF \<open>path M (initial M) p\<close>] 
+      unfolding completely_specified.simps by blast
   qed
   ultimately have ***: "(butlast ioF')@[(fst (last ioF'), t_output t)] \<in> L M"
   proof -
     have "p_io (p @ [t]) \<in> L M"
-      by (metis (no_types) \<open>path M (FSM.initial M) p\<close> \<open>t \<in> FSM.transitions M\<close> \<open>t_source t = target (FSM.initial M) p\<close> language_intro path_append single_transition_path)
+      by (metis (no_types) \<open>path M (FSM.initial M) p\<close> \<open>t \<in> FSM.transitions M\<close> \<open>t_source t = target (FSM.initial M) p\<close> 
+            language_intro path_append single_transition_path)
     then show ?thesis
       by (simp add: \<open>p_io p = butlast ioF'\<close> \<open>t_input t = fst (last ioF')\<close>)
   qed
 
-  show ?thesis using that[OF *** ** *] by assumption
-qed
-
-
-
-
-lemma language_append_path_ob :
-  assumes "io@[(x,y)] \<in> L M"
-  obtains p t where "path M (initial M) (p@[t])" and "p_io p = io" and "t_input t = x" and "t_output t = y"
-proof -
-  obtain p p2 where "path M (initial M) p" and "path M (target (initial M) p) p2"  and "p_io p = io" and "p_io p2 = [(x,y)]"
-    using language_state_split[OF assms] by blast
-
-  obtain t where "p2 = [t]" and "t_input t = x" and "t_output t = y"
-    using \<open>p_io p2 = [(x,y)]\<close> by auto
-
-  have "path M (initial M) (p@[t])"
-    using \<open>path M (initial M) p\<close> \<open>path M (target (initial M) p) p2\<close> unfolding \<open>p2 = [t]\<close> by auto
-  then show ?thesis using that[OF _ \<open>p_io p = io\<close> \<open>t_input t = x\<close> \<open>t_output t = y\<close>]
-    by simp 
+  show ?thesis 
+    using that[OF *** ** *] 
+    by assumption
 qed
 
 
@@ -400,34 +320,7 @@ proof -
 qed
 
 
-(* TODO: move *)
-lemma is_preamble_is_node : 
-  assumes "is_preamble P M q"
-  shows "q \<in> nodes M"
-  using assms unfolding is_preamble_def
-  by (meson nil path_nil_elim reachable_node_is_node submachine_path) 
 
-(* TODO: move *)
-lemma prefixes_set_ob :
-  assumes "xs \<in> set (prefixes xss)"
-  obtains xs' where "xss = xs@xs'"
-  using assms unfolding prefixes_set
-  by auto 
-
-(* TODO: move *)
-lemma language_finite: "finite {io . io \<in> L M \<and> length io \<le> k}"
-proof -
-  have "{io . io \<in> L M \<and> length io \<le> k} \<subseteq> p_io  ` {p. path M (FSM.initial M) p \<and> length p \<le> k}"
-    by auto
-  then show ?thesis
-    using paths_finite[of M "initial M" k]
-    using finite_surj by auto 
-qed
-
-
-
-(* TODO: remove assumptions *)
-(* TODO: remove superfluous tX *)
 lemma test_suite_to_io_pass :
   assumes "is_sufficient_for_reduction_testing T M m"
   and     "observable M" 
@@ -440,9 +333,6 @@ shows "pass_io_set M' (test_suite_to_io M T) = passes_test_suite M T M'"
 proof -
   obtain prs tps rd_targets atcs where "T = Test_Suite prs tps rd_targets atcs"
     by (meson test_suite.exhaust)
-
-
-
   then obtain RepSets where RepSets_def: "is_sufficient_for_reduction_testing_for_RepSets (Test_Suite prs tps rd_targets atcs) M m RepSets"
     using assms(1) unfolding is_sufficient_for_reduction_testing_def by blast
   then have "is_sufficient_for_reduction_testing (Test_Suite prs tps rd_targets atcs) M m"
@@ -452,17 +342,22 @@ proof -
 
 
   have t1: "(initial M, initial_preamble M) \<in> prs" 
-    using is_sufficient_for_reduction_testing_for_RepSets_simps(1)[OF RepSets_def] by assumption
+    using is_sufficient_for_reduction_testing_for_RepSets_simps(1)[OF RepSets_def] 
+    by assumption
   have t2: "\<And> q P. (q, P) \<in> prs \<Longrightarrow> is_preamble P M q"
-    using is_sufficient_for_reduction_testing_for_RepSets_simps(2)[OF RepSets_def] by blast
+    using is_sufficient_for_reduction_testing_for_RepSets_simps(2)[OF RepSets_def] 
+    by blast
   have t3: "\<And> q1 q2 A d1 d2. (A, d1, d2) \<in> atcs (q1, q2) \<Longrightarrow> (A, d2, d1) \<in> atcs (q2, q1) \<and> is_separator M q1 q2 A d1 d2"
-    using is_sufficient_for_reduction_testing_for_RepSets_simps(3)[OF RepSets_def] by assumption
+    using is_sufficient_for_reduction_testing_for_RepSets_simps(3)[OF RepSets_def] 
+    by assumption
   
   have t5: "\<And>q. q \<in> FSM.nodes M \<Longrightarrow> (\<exists>d\<in>set RepSets. q \<in> fst d)"
-    using is_sufficient_for_reduction_testing_for_RepSets_simps(4)[OF RepSets_def] by assumption
+    using is_sufficient_for_reduction_testing_for_RepSets_simps(4)[OF RepSets_def] 
+    by assumption
 
   have t6: "\<And> q. q \<in> fst ` prs \<Longrightarrow> tps q \<subseteq> {p1 . \<exists> p2 d . (p1@p2,d) \<in> m_traversal_paths_with_witness M q RepSets m} \<and> fst ` (m_traversal_paths_with_witness M q RepSets m) \<subseteq> tps q"
-    using is_sufficient_for_reduction_testing_for_RepSets_simps(7)[OF RepSets_def] by assumption
+    using is_sufficient_for_reduction_testing_for_RepSets_simps(7)[OF RepSets_def] 
+    by assumption
 
   have t7: "\<And> d. d \<in> set RepSets \<Longrightarrow> fst d \<subseteq> FSM.nodes M"
   and  t8: "\<And> d. d \<in> set RepSets \<Longrightarrow> snd d \<subseteq> fst d"
@@ -477,8 +372,8 @@ proof -
     assume "pass_io_set M' (test_suite_to_io M (Test_Suite prs tps rd_targets atcs))"
 
     then have pass_io_prop: "\<And> io x y y' . io @ [(x, y)] \<in> test_suite_to_io M (Test_Suite prs tps rd_targets atcs) \<Longrightarrow> io @ [(x, y')] \<in> L M' \<Longrightarrow> io @ [(x, y')] \<in> test_suite_to_io M (Test_Suite prs tps rd_targets atcs)"
-      unfolding pass_io_set_def by blast
-
+      unfolding pass_io_set_def 
+      by blast
 
     show "passes_test_suite M (Test_Suite prs tps rd_targets atcs) M'"
     proof (rule ccontr)
@@ -505,7 +400,10 @@ proof -
         unfolding passes_test_suite.simps by blast
       then show False proof cases
         case a
-        then obtain q P io x y y' where "(q, P) \<in> prs" and "io @ [(x, y)] \<in> L P" and "io @ [(x, y')] \<in> L M'" and "io @ [(x, y')] \<notin> L P"
+        then obtain q P io x y y' where "(q, P) \<in> prs" 
+                                    and "io @ [(x, y)] \<in> L P" 
+                                    and "io @ [(x, y')] \<in> L M'" 
+                                    and "io @ [(x, y')] \<notin> L P"
           by blast
 
         have "is_preamble P M q"
@@ -513,18 +411,23 @@ proof -
         
 
         have "io @ [(x, y)] \<in> test_suite_to_io M (Test_Suite prs tps rd_targets atcs)"
-          unfolding test_suite_to_io.simps using \<open>(q, P) \<in> prs\<close> \<open>io @ [(x, y)] \<in> L P\<close> by fastforce
+          unfolding test_suite_to_io.simps using \<open>(q, P) \<in> prs\<close> \<open>io @ [(x, y)] \<in> L P\<close>
+          by fastforce
 
         have "io @ [(x, y')] \<in> test_suite_to_io M (Test_Suite prs tps rd_targets atcs)"
-          using pass_io_prop[OF \<open>io @ [(x, y)] \<in> test_suite_to_io M (Test_Suite prs tps rd_targets atcs)\<close> \<open>io @ [(x, y')] \<in> L M'\<close>] by assumption
+          using pass_io_prop[OF \<open>io @ [(x, y)] \<in> test_suite_to_io M (Test_Suite prs tps rd_targets atcs)\<close> \<open>io @ [(x, y')] \<in> L M'\<close>] 
+          by assumption
 
         then have "io @ [(x, y')] \<in> L M"
-          using test_suite_language_prop by blast
+          using test_suite_language_prop 
+          by blast
 
         have "io @ [(x, y')] \<in> L P"
-          using passes_test_suite_soundness_helper_1[OF \<open>is_preamble P M q\<close> \<open>observable M\<close> \<open>io @ [(x, y)] \<in> L P\<close> \<open>io @ [(x, y')] \<in> L M\<close>] by assumption
+          using passes_test_suite_soundness_helper_1[OF \<open>is_preamble P M q\<close> \<open>observable M\<close> \<open>io @ [(x, y)] \<in> L P\<close> \<open>io @ [(x, y')] \<in> L M\<close>] 
+          by assumption
         then show "False"
-          using \<open>io @ [(x, y')] \<notin> L P\<close> by blast
+          using \<open>io @ [(x, y')] \<notin> L P\<close> 
+          by blast
 
       next
         case b
@@ -573,7 +476,9 @@ proof -
           by blast+
 
         obtain ioT' where "p_io pT = ioT @ [(x,y)] @ ioT'"
-          using prefixes_set_ob[OF \<open>ioT @ [(x, y)] \<in> set (prefixes (p_io pT))\<close>] unfolding prefixes_set append.assoc[symmetric] by blast
+          using prefixes_set_ob[OF \<open>ioT @ [(x, y)] \<in> set (prefixes (p_io pT))\<close>] 
+          unfolding prefixes_set append.assoc[symmetric] 
+          by blast
 
         let ?pt = "take (length (ioT @ [(x,y)])) pT"
         let ?p  = "butlast ?pt"
@@ -581,7 +486,9 @@ proof -
          
 
         have "length ?pt > 0"
-          using \<open>p_io pT = ioT @ [(x,y)] @ ioT'\<close> unfolding length_map[of "(\<lambda> t . (t_input t, t_output t))", symmetric] by auto
+          using \<open>p_io pT = ioT @ [(x,y)] @ ioT'\<close> 
+          unfolding length_map[of "(\<lambda> t . (t_input t, t_output t))", symmetric] 
+          by auto
         then have "?pt = ?p @ [?t]"
           by auto
         moreover have "path M q ?pt"
@@ -608,10 +515,16 @@ proof -
         then have "initial P = initial M" by auto
     
         have "path M (initial M) pP"
-          using submachine_path[OF \<open>is_submachine P M\<close> \<open>path P (initial P) pP\<close>] unfolding \<open>initial P = initial M\<close> by assumption
+          using submachine_path[OF \<open>is_submachine P M\<close> \<open>path P (initial P) pP\<close>] 
+          unfolding \<open>initial P = initial M\<close> 
+          by assumption
         moreover have "target (initial M) pP = q"
-          using \<open>target (initial P) pP = q\<close> unfolding \<open>initial P = initial M\<close> by assumption
-        ultimately have "path M (initial M) (pP@?p)" using \<open>path M q ?p\<close> by auto
+          using \<open>target (initial P) pP = q\<close> 
+          unfolding \<open>initial P = initial M\<close> 
+          by assumption
+        ultimately have "path M (initial M) (pP@?p)" 
+          using \<open>path M q ?p\<close> 
+          by auto
       
 
         have "find (\<lambda>d. Suc (m - card (snd d)) \<le> length (filter (\<lambda>t. t_target t \<in> fst d) ?p)) RepSets = None"
@@ -621,7 +534,9 @@ proof -
             by (metis append_assoc append_take_drop_id) 
           have **: "([?t] @ (drop (length (ioT @ [(x,y)])) pT) @ pT') \<noteq> []"
             by simp
-          show ?thesis using \<open>\<And> p' p''. (pT @ pT') = p' @ p'' \<Longrightarrow> p'' \<noteq> [] \<Longrightarrow> find (\<lambda>d. Suc (m - card (snd d)) \<le> length (filter (\<lambda>t. t_target t \<in> fst d) p')) RepSets = None\<close>[OF * **] by assumption
+          show ?thesis 
+            using \<open>\<And> p' p''. (pT @ pT') = p' @ p'' \<Longrightarrow> p'' \<noteq> [] \<Longrightarrow> find (\<lambda>d. Suc (m - card (snd d)) \<le> length (filter (\<lambda>t. t_target t \<in> fst d) p')) RepSets = None\<close>[OF * **] 
+            by assumption
         qed
 
 
@@ -630,7 +545,6 @@ proof -
           using language_append_path_ob[OF \<open>(p_io pP @ ioT) @ [(x, y')] \<in> L M\<close>] by blast
         then have "path M (FSM.initial M) p'" and "t_source t' = target (initial M) p'" and "t' \<in> transitions M"
           by auto
-
         
         have "p' = pP @ ?p"
           using observable_path_unique[OF \<open>observable M\<close> \<open>path M (FSM.initial M) p'\<close> \<open>path M (initial M) (pP@?p)\<close>] 
@@ -640,23 +554,29 @@ proof -
         then have "t_source t' = target q ?p"
           unfolding \<open>t_source t' = target (initial M) p'\<close> using \<open>target (initial M) pP = q\<close>
           by auto  
-        
-        
+                
         obtain pTt' dt' where "(?p @ [t'] @ pTt', dt') \<in> m_traversal_paths_with_witness M q RepSets m"
-          using m_traversal_path_extension_exist_for_transition[OF \<open>completely_specified M\<close> \<open>q \<in> nodes M\<close> \<open>FSM.inputs M \<noteq> {}\<close> t5 t8 \<open>path M q ?p\<close> \<open>find (\<lambda>d. Suc (m - card (snd d)) \<le> length (filter (\<lambda>t. t_target t \<in> fst d) ?p)) RepSets = None\<close> \<open>t' \<in> transitions M\<close> \<open>t_source t' = target q ?p\<close>]
+          using m_traversal_path_extension_exist_for_transition[OF \<open>completely_specified M\<close> \<open>q \<in> nodes M\<close> \<open>FSM.inputs M \<noteq> {}\<close> 
+                                                                   t5 t8 \<open>path M q ?p\<close> \<open>find (\<lambda>d. Suc (m - card (snd d)) \<le> length (filter (\<lambda>t. t_target t \<in> fst d) ?p)) RepSets = None\<close> 
+                                                                   \<open>t' \<in> transitions M\<close> \<open>t_source t' = target q ?p\<close>]
           by blast
 
         have "?p @ [t'] @ pTt' \<in> tps q"
-          using t6[OF \<open>q \<in> fst ` prs\<close> ] \<open>(?p @ [t'] @ pTt', dt') \<in> m_traversal_paths_with_witness M q RepSets m\<close> by force
+          using t6[OF \<open>q \<in> fst ` prs\<close> ] \<open>(?p @ [t'] @ pTt', dt') \<in> m_traversal_paths_with_witness M q RepSets m\<close>
+          by force
         moreover have "ioT @ [(x, y')] \<in> set (prefixes (p_io (?p @ [t'] @ pTt')))"
         proof -
           have "p_io (?p @ [t'] @ pTt') = ioT @ [(x,y')] @ p_io pTt'"
-            using \<open>p_io ?p = ioT\<close> using \<open>t_input t' = x\<close> \<open>t_output t' = y'\<close> by auto  
-          then show ?thesis unfolding prefixes_set by force
+            using \<open>p_io ?p = ioT\<close> using \<open>t_input t' = x\<close> \<open>t_output t' = y'\<close> 
+            by auto  
+          then show ?thesis 
+            unfolding prefixes_set
+            by force
         qed
 
         ultimately show "False"
-          using \<open>\<not> (\<exists>pT'. pT' \<in> tps q \<and> ioT @ [(x, y')] \<in> set (prefixes (p_io pT')))\<close> by blast
+          using \<open>\<not> (\<exists>pT'. pT' \<in> tps q \<and> ioT @ [(x, y')] \<in> set (prefixes (p_io pT')))\<close> 
+          by blast
       next
         case c
 
@@ -673,16 +593,23 @@ proof -
 
 
         have "is_submachine P M"
-          using t2[OF \<open>(q, P) \<in> prs\<close>] unfolding is_preamble_def by blast
+          using t2[OF \<open>(q, P) \<in> prs\<close>] 
+          unfolding is_preamble_def 
+          by blast
         then have "initial P = initial M" by auto
     
         have "path M (initial M) pP"
-          using submachine_path[OF \<open>is_submachine P M\<close> \<open>path P (initial P) pP\<close>] unfolding \<open>initial P = initial M\<close> by assumption
+          using submachine_path[OF \<open>is_submachine P M\<close> \<open>path P (initial P) pP\<close>] 
+          unfolding \<open>initial P = initial M\<close> 
+          by assumption
         have "target (initial M) pP = q"
-          using \<open>target (initial P) pP = q\<close> unfolding \<open>initial P = initial M\<close> by assumption
+          using \<open>target (initial P) pP = q\<close> 
+          unfolding \<open>initial P = initial M\<close> 
+          by assumption
 
         have "q \<in> nodes M"
-          using is_preamble_is_node[OF t2[OF \<open>(q, P) \<in> prs\<close>]] by assumption
+          using is_preamble_is_node[OF t2[OF \<open>(q, P) \<in> prs\<close>]] 
+          by assumption
 
         have "q \<in> fst ` prs" 
           using \<open>(q, P) \<in> prs\<close> by force
@@ -699,8 +626,8 @@ proof -
           by auto
 
         have "qT \<in> nodes M'"
-          using \<open>qT \<in> io_targets M' (p_io pP @ p_io pT) (FSM.initial M')\<close> io_targets_nodes
-          using subset_iff by fastforce 
+          using \<open>qT \<in> io_targets M' (p_io pP @ p_io pT) (FSM.initial M')\<close> io_targets_nodes subset_iff 
+          by fastforce 
 
 
 
@@ -709,7 +636,9 @@ proof -
 
         have "\<not> pass_io_set (FSM.from_FSM M' qT) (atc_to_io_set (FSM.from_FSM M (target q pT)) A)"
           using \<open>\<not>pass_separator_ATC M' A qT d2\<close>
-                pass_separator_pass_io_set_iff[OF \<open>is_separator M (target q pT) q' A d1 d2\<close> \<open>observable M\<close> \<open>observable M'\<close> path_target_is_node[OF \<open>path M q pT\<close>] \<open>qT \<in> nodes M'\<close> \<open>inputs M' = inputs M\<close> \<open>completely_specified M\<close>]
+                pass_separator_pass_io_set_iff[OF \<open>is_separator M (target q pT) q' A d1 d2\<close> \<open>observable M\<close> 
+                                                  \<open>observable M'\<close> path_target_is_node[OF \<open>path M q pT\<close>] 
+                                                  \<open>qT \<in> nodes M'\<close> \<open>inputs M' = inputs M\<close> \<open>completely_specified M\<close>]
           by simp
 
 
@@ -739,13 +668,12 @@ proof -
             then have *: "(p_io pP @ p_io pT @ io) @ [(x, y)] \<in> test_suite_to_io M (Test_Suite prs tps rd_targets atcs)"
               by simp
 
-
             have "io @ [(x, y')] \<in> LS M' qT"
               using \<open>io @ [(x, y')] \<in> L (FSM.from_FSM M' qT)\<close> \<open>qT \<in> nodes M'\<close>
               by (metis from_FSM_language) 
             have **: "(p_io pP @ p_io pT @ io) @ [(x, y')] \<in> L M'" 
-              using io_targets_language_append[OF \<open>qT \<in> io_targets M' (p_io pP @ p_io pT) (FSM.initial M')\<close> \<open>io @ [(x, y')] \<in> LS M' qT\<close>] by simp
-            
+              using io_targets_language_append[OF \<open>qT \<in> io_targets M' (p_io pP @ p_io pT) (FSM.initial M')\<close> \<open>io @ [(x, y')] \<in> LS M' qT\<close>] 
+              by simp            
             
             have "(p_io pP @ p_io pT) @ (io @ [(x, y')]) \<in> test_suite_to_io M (Test_Suite prs tps rd_targets atcs)"
               using pass_io_prop[OF * ** ] by simp
@@ -757,7 +685,8 @@ proof -
               have "target (initial M) (pP@pT) = target q pT"
                 unfolding \<open>target (initial M) pP = q\<close>[symmetric] by auto
               moreover have "path M (initial M) (pP@pT)"
-                using \<open>path M (initial M) pP\<close> \<open>path M q pT\<close> unfolding \<open>target (initial M) pP = q\<close>[symmetric] by auto
+                using \<open>path M (initial M) pP\<close> \<open>path M q pT\<close> unfolding \<open>target (initial M) pP = q\<close>[symmetric] 
+                by auto
               moreover have "p_io (pP@pT) = (p_io pP @ p_io pT)" 
                 by auto
               ultimately show ?thesis
@@ -766,15 +695,15 @@ proof -
             qed
 
             ultimately have "io @ [(x, y')] \<in> LS M (target q pT)"
-              using observable_io_targets_language[OF _ \<open>observable M\<close>, of "(p_io pP @ p_io pT)" "(io @ [(x, y')])" "initial M" "target q pT"] by blast
-
-
-            
+              using observable_io_targets_language[OF _ \<open>observable M\<close>, of "(p_io pP @ p_io pT)" "(io @ [(x, y')])" "initial M" "target q pT"] 
+              by blast            
             then have "io @ [(x, y')] \<in> L (FSM.from_FSM M (target q pT))"
-              unfolding from_FSM_language[OF path_target_is_node[OF \<open>path M q pT\<close>]] by assumption
+              unfolding from_FSM_language[OF path_target_is_node[OF \<open>path M q pT\<close>]] 
+              by assumption
 
             moreover have "io @ [(x, y')] \<in> L A"
-              by (metis Int_iff \<open>io @ [(x, y')] \<in> LS M (target q pT)\<close> \<open>io @ [(x, y)] \<in> atc_to_io_set (FSM.from_FSM M (target q pT)) A\<close> \<open>is_separator M (target q pT) q' A d1 d2\<close> atc_to_io_set.simps is_separator_simps(9))
+              by (metis Int_iff \<open>io @ [(x, y')] \<in> LS M (target q pT)\<close> \<open>io @ [(x, y)] \<in> atc_to_io_set (FSM.from_FSM M (target q pT)) A\<close> 
+                      \<open>is_separator M (target q pT) q' A d1 d2\<close> atc_to_io_set.simps is_separator_simps(9))
               
             ultimately show "io @ [(x, y')] \<in> atc_to_io_set (FSM.from_FSM M (target q pT)) A"
               unfolding atc_to_io_set.simps by blast
@@ -784,7 +713,9 @@ proof -
         qed
 
         then show "False"
-          using pass_separator_from_pass_io_set[OF \<open>is_separator M (target q pT) q' A d1 d2\<close> _ \<open>observable M\<close> \<open>observable M'\<close> path_target_is_node[OF \<open>path M q pT\<close>] \<open>qT \<in> nodes M'\<close> \<open>inputs M' = inputs M\<close> \<open>completely_specified M\<close>]
+          using pass_separator_from_pass_io_set[OF \<open>is_separator M (target q pT) q' A d1 d2\<close> _ \<open>observable M\<close> 
+                                                   \<open>observable M'\<close> path_target_is_node[OF \<open>path M q pT\<close>] 
+                                                   \<open>qT \<in> nodes M'\<close> \<open>inputs M' = inputs M\<close> \<open>completely_specified M\<close>]
                 \<open>\<not>pass_separator_ATC M' A qT d2\<close>
           by simp
       qed
@@ -825,10 +756,12 @@ proof -
       have preamble_prop: "\<And> q P . (q, P) \<in> prs \<Longrightarrow> io @ [(x, y)] \<in> L P \<Longrightarrow> False"
       proof - 
         fix q P assume "(q, P)\<in>prs" and "io @ [(x, y)] \<in> L P" 
-        have "io @ [(x, y')] \<in> L P" using pass1[OF \<open>(q, P)\<in>prs\<close> \<open>io @ [(x, y)] \<in> L P\<close> \<open>io @ [(x, y')] \<in> L M'\<close> ] by assumption
+        have "io @ [(x, y')] \<in> L P" using pass1[OF \<open>(q, P)\<in>prs\<close> \<open>io @ [(x, y)] \<in> L P\<close> \<open>io @ [(x, y')] \<in> L M'\<close> ] 
+          by assumption
         then have "io @ [(x, y')] \<in> test_suite_to_io M (Test_Suite prs tps rd_targets atcs)"
           unfolding test_suite_to_io.simps using \<open>(q, P)\<in>prs\<close> by blast
-        then show "False" using \<open>io @ [(x, y')] \<notin> test_suite_to_io M (Test_Suite prs tps rd_targets atcs)\<close> by simp
+        then show "False" using \<open>io @ [(x, y')] \<notin> test_suite_to_io M (Test_Suite prs tps rd_targets atcs)\<close> 
+          by simp
       qed
 
       have traversal_path_prop : "\<And> pP pt q P .  io @ [(x, y)] \<in> (@) (p_io pP) ` set (prefixes (p_io pt)) \<Longrightarrow> (q, P) \<in> prs \<Longrightarrow> path P (FSM.initial P) pP \<Longrightarrow> target (FSM.initial P) pP = q \<Longrightarrow> pt \<in> tps q \<Longrightarrow> False"
@@ -840,21 +773,30 @@ proof -
                        and   "pt \<in> tps q"
 
         obtain io' io'' where "io @ [(x, y)] = (p_io pP) @ io'" and "io'@io'' = p_io pt"
-          using \<open>io @ [(x, y)] \<in> (@) (p_io pP) ` set (prefixes (p_io pt))\<close> unfolding prefixes_set
+          using \<open>io @ [(x, y)] \<in> (@) (p_io pP) ` set (prefixes (p_io pt))\<close> 
+          unfolding prefixes_set
           by blast 
 
 
         have "is_submachine P M"
-          using t2[OF \<open>(q, P) \<in> prs\<close>] unfolding is_preamble_def by blast
-        then have "initial P = initial M" by auto
+          using t2[OF \<open>(q, P) \<in> prs\<close>] 
+          unfolding is_preamble_def 
+          by blast
+        then have "initial P = initial M" 
+          by auto
     
         have "path M (initial M) pP"
-          using submachine_path[OF \<open>is_submachine P M\<close> \<open>path P (initial P) pP\<close>] unfolding \<open>initial P = initial M\<close> by assumption
+          using submachine_path[OF \<open>is_submachine P M\<close> \<open>path P (initial P) pP\<close>] 
+          unfolding \<open>initial P = initial M\<close> 
+          by assumption
         have "target (initial M) pP = q"
-          using \<open>target (initial P) pP = q\<close> unfolding \<open>initial P = initial M\<close> by assumption
+          using \<open>target (initial P) pP = q\<close> 
+          unfolding \<open>initial P = initial M\<close> 
+          by assumption
 
         have "q \<in> nodes M"
-          using is_preamble_is_node[OF t2[OF \<open>(q, P) \<in> prs\<close>]] by assumption
+          using is_preamble_is_node[OF t2[OF \<open>(q, P) \<in> prs\<close>]] 
+          by assumption
 
         have "q \<in> fst ` prs" 
           using \<open>(q, P) \<in> prs\<close> by force
@@ -862,9 +804,12 @@ proof -
 
         show "False" proof (cases io' rule: rev_cases)
           case Nil
-          then have "p_io pP = io @ [(x, y)]" using \<open>io @ [(x, y)] = (p_io pP) @ io'\<close> by auto
+          then have "p_io pP = io @ [(x, y)]" 
+            using \<open>io @ [(x, y)] = (p_io pP) @ io'\<close>
+            by auto
           show ?thesis
-            using preamble_prop[OF \<open>(q,P) \<in> prs\<close> language_state_containment[OF \<open>path P (FSM.initial P) pP\<close> \<open>p_io pP = io @ [(x, y)]\<close>]] by assumption
+            using preamble_prop[OF \<open>(q,P) \<in> prs\<close> language_state_containment[OF \<open>path P (FSM.initial P) pP\<close> \<open>p_io pP = io @ [(x, y)]\<close>]]
+            by assumption
         next
           case (snoc ioI xy)
           then have "xy = (x,y)" and "io = (p_io pP) @ ioI"
@@ -874,28 +819,32 @@ proof -
 
           have "ioI @ [(x, y)] \<in> set (prefixes (p_io pt))"
             unfolding prefixes_set
-            using \<open>io' @ io'' = p_io pt\<close> \<open>xy = (x, y)\<close> snoc by auto 
+            using \<open>io' @ io'' = p_io pt\<close> \<open>xy = (x, y)\<close> snoc 
+            by auto 
 
           obtain pT' where "pT' \<in> tps q" and "ioI @ [(x, y')] \<in> set (prefixes (p_io pT'))"
-            using pass2[OF \<open>(q, P) \<in> prs\<close> \<open>path P (FSM.initial P) pP\<close> \<open>target (FSM.initial P) pP = q\<close> \<open>pt \<in> tps q\<close> \<open>ioI @ [(x, y)] \<in> set (prefixes (p_io pt))\<close> \<open>p_io pP @ ioI @ [(x, y')] \<in> L M'\<close>] by blast
+            using pass2[OF \<open>(q, P) \<in> prs\<close> \<open>path P (FSM.initial P) pP\<close> \<open>target (FSM.initial P) pP = q\<close> \<open>pt \<in> tps q\<close>
+                           \<open>ioI @ [(x, y)] \<in> set (prefixes (p_io pt))\<close> \<open>p_io pP @ ioI @ [(x, y')] \<in> L M'\<close>] by blast
 
           have "io @ [(x, y')] \<in> (@) (p_io pP) ` set (prefixes (p_io pT'))"
-            using \<open>ioI @ [(x, y')] \<in> set (prefixes (p_io pT'))\<close> unfolding \<open>io = (p_io pP) @ ioI\<close>
+            using \<open>ioI @ [(x, y')] \<in> set (prefixes (p_io pT'))\<close> 
+            unfolding \<open>io = (p_io pP) @ ioI\<close>
             by simp
 
           
           have "io @ [(x, y')] \<in> (\<Union> {(@) (p_io p) ` set (prefixes (p_io pt)) |p pt. \<exists>q P. (q, P) \<in> prs \<and> path P (FSM.initial P) p \<and> target (FSM.initial P) p = q \<and> pt \<in> tps q})"
-            using \<open>(q, P) \<in> prs\<close> \<open>path P (FSM.initial P) pP\<close> \<open>target (FSM.initial P) pP = q\<close> \<open>pT' \<in> tps q\<close> \<open>io @ [(x, y')] \<in> (@) (p_io pP) ` set (prefixes (p_io pT'))\<close> by blast
+            using \<open>(q, P) \<in> prs\<close> \<open>path P (FSM.initial P) pP\<close> \<open>target (FSM.initial P) pP = q\<close> 
+                  \<open>pT' \<in> tps q\<close> \<open>io @ [(x, y')] \<in> (@) (p_io pP) ` set (prefixes (p_io pT'))\<close> 
+            by blast
           then have "io @ [(x, y')] \<in> test_suite_to_io M (Test_Suite prs tps rd_targets atcs)"
-            unfolding test_suite_to_io.simps by blast
+            unfolding test_suite_to_io.simps 
+            by blast
 
           then show "False"
-            using \<open>io @ [(x, y')] \<notin> test_suite_to_io M (Test_Suite prs tps rd_targets atcs)\<close> by blast
+            using \<open>io @ [(x, y')] \<notin> test_suite_to_io M (Test_Suite prs tps rd_targets atcs)\<close> 
+            by blast
         qed
       qed
-
-
-
 
       consider (a) "io @ [(x, y)] \<in> (\<Union>(q, P)\<in>prs. L P)" |
                (b) "io @ [(x, y)] \<in> (\<Union> {(@) (p_io p) ` set (prefixes (p_io pt)) |p pt. \<exists>q P. (q, P) \<in> prs \<and> path P (FSM.initial P) p \<and> target (FSM.initial P) p = q \<and> pt \<in> tps q})" |
@@ -925,10 +874,9 @@ proof -
           by blast
 
         obtain ioA where "io @ [(x, y)] = p_io pP @ p_io pt @ ioA"
-          using \<open>io @ [(x, y)] \<in> (\<lambda>io_atc. p_io pP @ p_io pt @ io_atc) ` atc_to_io_set (FSM.from_FSM M (target q pt)) A\<close> unfolding prefixes_set
+          using \<open>io @ [(x, y)] \<in> (\<lambda>io_atc. p_io pP @ p_io pt @ io_atc) ` atc_to_io_set (FSM.from_FSM M (target q pt)) A\<close> 
+          unfolding prefixes_set
           by blast 
-
-
 
         show "False" proof (cases ioA rule: rev_cases)
           case Nil
@@ -937,20 +885,23 @@ proof -
           then have "io @ [(x, y)] \<in> (@) (p_io pP) ` set (prefixes (p_io pt))"
             unfolding prefixes_set by blast
           show ?thesis 
-            using traversal_path_prop[OF \<open>io @ [(x, y)] \<in> (@) (p_io pP) ` set (prefixes (p_io pt))\<close> \<open>(q, P) \<in> prs\<close> \<open>path P (FSM.initial P) pP\<close> \<open>target (FSM.initial P) pP = q\<close> \<open>pt \<in> tps q\<close>]
+            using traversal_path_prop[OF \<open>io @ [(x, y)] \<in> (@) (p_io pP) ` set (prefixes (p_io pt))\<close> \<open>(q, P) \<in> prs\<close> 
+                                         \<open>path P (FSM.initial P) pP\<close> \<open>target (FSM.initial P) pP = q\<close> \<open>pt \<in> tps q\<close>]
             by assumption
         next
           case (snoc ioAI xy)
           then have "xy = (x,y)" and "io = p_io pP @ p_io pt @ ioAI"
             using \<open>io @ [(x, y)] = p_io pP @ p_io pt @ ioA\<close> by simp+
           then have "p_io pP @ p_io pt @ ioAI @ [(x,y)] \<in> (\<lambda>io_atc. p_io pP @ p_io pt @ io_atc) ` atc_to_io_set (FSM.from_FSM M (target q pt)) A"
-            using \<open>io @ [(x, y)] \<in> (\<lambda>io_atc. p_io pP @ p_io pt @ io_atc) ` atc_to_io_set (FSM.from_FSM M (target q pt)) A\<close> by auto
+            using \<open>io @ [(x, y)] \<in> (\<lambda>io_atc. p_io pP @ p_io pt @ io_atc) ` atc_to_io_set (FSM.from_FSM M (target q pt)) A\<close> 
+            by auto
           then have "ioAI @ [(x,y)] \<in> atc_to_io_set (FSM.from_FSM M (target q pt)) A" 
             by auto
 
 
           have "p_io pP @ p_io pt \<in> L M'"
-            using \<open>io @ [(x,y')] \<in> L M'\<close> language_prefix[of "p_io pP @ p_io pt" "ioAI @ [(x, y')]" M' "initial M'"] unfolding \<open>io = p_io pP @ p_io pt @ ioAI\<close>
+            using \<open>io @ [(x,y')] \<in> L M'\<close> language_prefix[of "p_io pP @ p_io pt" "ioAI @ [(x, y')]" M' "initial M'"] 
+            unfolding \<open>io = p_io pP @ p_io pt @ ioAI\<close>
             by simp
           then obtain pt' where "path M' (initial M') pt'" and "p_io pt' = p_io pP @ p_io pt"
             by auto
@@ -959,30 +910,37 @@ proof -
               
             
           have "pass_separator_ATC M' A (target (FSM.initial M') pt') t2"
-            using pass3[OF \<open>(q, P) \<in> prs\<close> \<open>path P (FSM.initial P) pP\<close> \<open>target (FSM.initial P) pP = q\<close> \<open>pt \<in> tps q\<close> \<open>p_io pP @ p_io pt \<in> L M'\<close> \<open>q' \<in> rd_targets (q, pt)\<close> \<open>(A, t1, t2) \<in> atcs (target q pt, q')\<close> \<open>target (initial M') pt' \<in> io_targets M' (p_io pP @ p_io pt) (FSM.initial M')\<close>]
+            using pass3[OF \<open>(q, P) \<in> prs\<close> \<open>path P (FSM.initial P) pP\<close> \<open>target (FSM.initial P) pP = q\<close> \<open>pt \<in> tps q\<close> 
+                           \<open>p_io pP @ p_io pt \<in> L M'\<close> \<open>q' \<in> rd_targets (q, pt)\<close> \<open>(A, t1, t2) \<in> atcs (target q pt, q')\<close> 
+                           \<open>target (initial M') pt' \<in> io_targets M' (p_io pP @ p_io pt) (FSM.initial M')\<close>]
             by assumption
 
           have "is_separator M (target q pt) q' A t1 t2"
             using  t3[OF \<open>(A, t1, t2) \<in> atcs (target q pt, q')\<close>] by blast
-
 
           have "is_submachine P M"
             using t2[OF \<open>(q, P) \<in> prs\<close>] unfolding is_preamble_def by blast
           then have "initial P = initial M" by auto
       
           have "path M (initial M) pP"
-            using submachine_path[OF \<open>is_submachine P M\<close> \<open>path P (initial P) pP\<close>] unfolding \<open>initial P = initial M\<close> by assumption
+            using submachine_path[OF \<open>is_submachine P M\<close> \<open>path P (initial P) pP\<close>] 
+            unfolding \<open>initial P = initial M\<close> 
+            by assumption
           have "target (initial M) pP = q"
-            using \<open>target (initial P) pP = q\<close> unfolding \<open>initial P = initial M\<close> by assumption
+            using \<open>target (initial P) pP = q\<close> 
+            unfolding \<open>initial P = initial M\<close> 
+            by assumption
   
           have "q \<in> nodes M"
-            using is_preamble_is_node[OF t2[OF \<open>(q, P) \<in> prs\<close>]] by assumption
+            using is_preamble_is_node[OF t2[OF \<open>(q, P) \<in> prs\<close>]] 
+            by assumption
   
           have "q \<in> fst ` prs" 
             using \<open>(q, P) \<in> prs\<close> by force
   
           obtain pT' d' where "(pt @ pT', d') \<in> m_traversal_paths_with_witness M q RepSets m"
-            using t6[OF \<open>q \<in> fst ` prs\<close>] \<open>pt \<in> tps q\<close> by blast
+            using t6[OF \<open>q \<in> fst ` prs\<close>] \<open>pt \<in> tps q\<close> 
+            by blast
   
           then have "path M q (pt @ pT')"
                and  "find (\<lambda>d. Suc (m - card (snd d)) \<le> length (filter (\<lambda>t. t_target t \<in> fst d) (pt @ pT'))) RepSets = Some d'"
@@ -994,16 +952,22 @@ proof -
   
           have "target (initial M') pt' \<in> nodes M'"
             using \<open>target (initial M') pt' \<in> io_targets M' (p_io pP @ p_io pt) (FSM.initial M')\<close> io_targets_nodes
-            using subset_iff by fastforce 
+            using subset_iff 
+            by fastforce 
 
 
           have "pass_io_set (FSM.from_FSM M' (target (FSM.initial M') pt')) (atc_to_io_set (FSM.from_FSM M (target q pt)) A)"
-            using  pass_io_set_from_pass_separator[OF \<open>is_separator M (target q pt) q' A t1 t2\<close> \<open>pass_separator_ATC M' A (target (FSM.initial M') pt') t2\<close> \<open>observable M\<close> \<open>observable M'\<close> path_target_is_node[OF \<open>path M q pt\<close>] \<open>target (FSM.initial M') pt' \<in> FSM.nodes M'\<close> \<open>inputs M' = inputs M\<close>]
+            using  pass_io_set_from_pass_separator[OF \<open>is_separator M (target q pt) q' A t1 t2\<close> 
+                                                      \<open>pass_separator_ATC M' A (target (FSM.initial M') pt') t2\<close> 
+                                                      \<open>observable M\<close> \<open>observable M'\<close> path_target_is_node[OF \<open>path M q pt\<close>] 
+                                                      \<open>target (FSM.initial M') pt' \<in> FSM.nodes M'\<close> \<open>inputs M' = inputs M\<close>]
             by assumption
           moreover note \<open>ioAI @ [(x,y)] \<in> atc_to_io_set (FSM.from_FSM M (target q pt)) A\<close>
           moreover have "ioAI @ [(x, y')] \<in> L (FSM.from_FSM M' (target (FSM.initial M') pt'))" 
             using \<open>io @ [(x,y')] \<in> L M'\<close>   unfolding \<open>io = p_io pP @ p_io pt @ ioAI\<close>
-            by (metis (no_types, lifting) \<open>target (FSM.initial M') pt' \<in> FSM.nodes M'\<close> \<open>target (FSM.initial M') pt' \<in> io_targets M' (p_io pP @ p_io pt) (FSM.initial M')\<close> append_assoc assms(3) from_FSM_language observable_io_targets_language)
+            by (metis (no_types, lifting) \<open>target (FSM.initial M') pt' \<in> FSM.nodes M'\<close> 
+                  \<open>target (FSM.initial M') pt' \<in> io_targets M' (p_io pP @ p_io pt) (FSM.initial M')\<close> 
+                  append_assoc assms(3) from_FSM_language observable_io_targets_language)
 
           ultimately have "ioAI @ [(x,y')] \<in> atc_to_io_set (FSM.from_FSM M (target q pt)) A"
             unfolding pass_io_set_def by blast
@@ -1025,20 +989,17 @@ proof -
           then have "io @ [(x, y')] \<in> test_suite_to_io M (Test_Suite prs tps rd_targets atcs)"
             unfolding \<open>io = p_io pP @ p_io pt @ ioAI\<close> by auto
           then show "False"
-            using \<open>io @ [(x, y')] \<notin> test_suite_to_io M (Test_Suite prs tps rd_targets atcs)\<close> by blast
+            using \<open>io @ [(x, y')] \<notin> test_suite_to_io M (Test_Suite prs tps rd_targets atcs)\<close> 
+            by blast
         qed
       qed
     qed
   qed
 
   ultimately show ?thesis 
-    unfolding \<open>T = Test_Suite prs tps rd_targets atcs\<close> by blast
+    unfolding \<open>T = Test_Suite prs tps rd_targets atcs\<close> 
+    by blast
 qed
-
-
-
-
-subsubsection \<open>Using Maximal Sequences Only\<close>
 
 
 
@@ -1049,36 +1010,41 @@ shows "finite (test_suite_to_io M T)"
 proof -
   obtain prs tps rd_targets atcs where "T = Test_Suite prs tps rd_targets atcs"
     by (meson test_suite.exhaust)
-
-
-
   then obtain RepSets where RepSets_def: "is_sufficient_for_reduction_testing_for_RepSets (Test_Suite prs tps rd_targets atcs) M m RepSets"
-    using assms(1) unfolding is_sufficient_for_reduction_testing_def by blast
+    using assms(1) 
+    unfolding is_sufficient_for_reduction_testing_def 
+    by blast
   then have "is_sufficient_for_reduction_testing (Test_Suite prs tps rd_targets atcs) M m"
-    unfolding is_sufficient_for_reduction_testing_def by blast
+    unfolding is_sufficient_for_reduction_testing_def 
+    by blast
   then have test_suite_language_prop: "test_suite_to_io M (Test_Suite prs tps rd_targets atcs) \<subseteq> L M"
-    using test_suite_to_io_language by blast
-
+    using test_suite_to_io_language 
+    by blast
 
   have f1: "(finite prs)" 
   and  f2: "\<And> q p . q \<in> fst ` prs \<Longrightarrow> finite (rd_targets (q,p))" 
   and  f3: "\<And> q q' . finite (atcs (q,q'))"
-    using assms(2) unfolding \<open>T = Test_Suite prs tps rd_targets atcs\<close> is_finite_test_suite.simps by blast+
-
-
+    using assms(2) 
+    unfolding \<open>T = Test_Suite prs tps rd_targets atcs\<close> is_finite_test_suite.simps 
+    by blast+
 
   have t1: "(initial M, initial_preamble M) \<in> prs" 
-    using is_sufficient_for_reduction_testing_for_RepSets_simps(1)[OF RepSets_def] by assumption
+    using is_sufficient_for_reduction_testing_for_RepSets_simps(1)[OF RepSets_def] 
+    by assumption
   have t2: "\<And> q P. (q, P) \<in> prs \<Longrightarrow> is_preamble P M q"
-    using is_sufficient_for_reduction_testing_for_RepSets_simps(2)[OF RepSets_def] by blast
+    using is_sufficient_for_reduction_testing_for_RepSets_simps(2)[OF RepSets_def] 
+    by blast
   have t3: "\<And> q1 q2 A d1 d2. (A, d1, d2) \<in> atcs (q1, q2) \<Longrightarrow> (A, d2, d1) \<in> atcs (q2, q1) \<and> is_separator M q1 q2 A d1 d2"
-    using is_sufficient_for_reduction_testing_for_RepSets_simps(3)[OF RepSets_def] by assumption
+    using is_sufficient_for_reduction_testing_for_RepSets_simps(3)[OF RepSets_def] 
+    by assumption
   
   have t5: "\<And>q. q \<in> FSM.nodes M \<Longrightarrow> (\<exists>d\<in>set RepSets. q \<in> fst d)"
-    using is_sufficient_for_reduction_testing_for_RepSets_simps(4)[OF RepSets_def] by assumption
+    using is_sufficient_for_reduction_testing_for_RepSets_simps(4)[OF RepSets_def] 
+    by assumption
 
   have t6: "\<And> q. q \<in> fst ` prs \<Longrightarrow> tps q \<subseteq> {p1 . \<exists> p2 d . (p1@p2,d) \<in> m_traversal_paths_with_witness M q RepSets m} \<and> fst ` (m_traversal_paths_with_witness M q RepSets m) \<subseteq> tps q"
-    using is_sufficient_for_reduction_testing_for_RepSets_simps(7)[OF RepSets_def] by assumption
+    using is_sufficient_for_reduction_testing_for_RepSets_simps(7)[OF RepSets_def] 
+    by assumption
 
   have t7: "\<And> d. d \<in> set RepSets \<Longrightarrow> fst d \<subseteq> FSM.nodes M"
   and  t8: "\<And> d. d \<in> set RepSets \<Longrightarrow> snd d \<subseteq> fst d"
@@ -1116,10 +1082,6 @@ proof -
   then have f4' : "\<And> q P . (q,P) \<in> prs \<Longrightarrow> finite (tps q)"
     by force
 
-
-
-
-
   define T1 where T1_def : "T1 = (\<Union>(q, P)\<in>prs. L P)"
   define T2 where T2_def : "T2 = \<Union>{(@) (p_io p) ` set (prefixes (p_io pt)) |p pt. \<exists>q P. (q, P) \<in> prs \<and> path P (FSM.initial P) p \<and> target (FSM.initial P) p = q \<and> pt \<in> tps q}"
   define T3 where T3_def : "T3 = \<Union> {(\<lambda>io_atc. p_io p @ p_io pt @ io_atc) ` atc_to_io_set (FSM.from_FSM M (target q pt)) A |p pt q A.
@@ -1135,8 +1097,13 @@ proof -
     have "\<And> q P . (q, P)\<in>prs \<Longrightarrow> finite (L P)"
     proof -
       fix q P assume "(q, P)\<in>prs"
-      have "acyclic P" using t2[OF \<open>(q, P)\<in>prs\<close>] unfolding is_preamble_def by blast 
-      then show "finite (L P)" using acyclic_alt_def by blast
+      have "acyclic P" 
+        using t2[OF \<open>(q, P)\<in>prs\<close>] 
+        unfolding is_preamble_def 
+        by blast 
+      then show "finite (L P)" 
+        using acyclic_alt_def 
+        by blast
     qed
     then show ?thesis using f1 unfolding T1_def
       by auto 
@@ -1145,8 +1112,8 @@ proof -
   moreover have "finite T2"
   proof -
     have *: "T2 = (\<Union> (p,pt) \<in> {(p,pt) | p pt. \<exists>q P. (q, P) \<in> prs \<and> path P (FSM.initial P) p \<and> target (FSM.initial P) p = q \<and> pt \<in> tps q} . ((@) (p_io p) ` set (prefixes (p_io pt))))"
-      unfolding T2_def by auto
-
+      unfolding T2_def 
+      by auto
 
     have "\<And> p pt . finite ((@) (p_io p) ` set (prefixes (p_io pt)))"
       by auto
@@ -1161,24 +1128,32 @@ proof -
         proof -
           fix q P assume "(q,P) \<in> prs"
 
-          have "acyclic P" using t2[OF \<open>(q, P)\<in>prs\<close>] unfolding is_preamble_def by blast
-          then have "finite {p . path P (initial P) p}" using acyclic_paths_finite[of P "initial P"] unfolding acyclic.simps
+          have "acyclic P" using t2[OF \<open>(q, P)\<in>prs\<close>]
+            unfolding is_preamble_def 
+            by blast
+          then have "finite {p . path P (initial P) p}" 
+            using acyclic_paths_finite[of P "initial P"] 
+            unfolding acyclic.simps
             by (metis (no_types, lifting) Collect_cong) 
           then show "finite ({p . path P (initial P) p} \<times> (tps q))"
-            using f4'[OF \<open>(q,P) \<in> prs\<close>] by simp
+            using f4'[OF \<open>(q,P) \<in> prs\<close>] 
+            by simp
         qed
-        ultimately show ?thesis by force
+        ultimately show ?thesis 
+          by force
       qed
       ultimately show ?thesis
         by (meson rev_finite_subset) 
     qed
-    ultimately show ?thesis unfolding * by auto 
+    ultimately show ?thesis 
+      unfolding * by auto 
   qed
 
 
   moreover have "finite T3"
   proof -
-    have scheme: "\<And> f P . (\<Union> {f a b c d | a b c d . P a b c d}) = (\<Union> (a,b,c,d) \<in> {(a,b,c,d) | a b c d . P a b c d} . f a b c d)" by blast
+    have scheme: "\<And> f P . (\<Union> {f a b c d | a b c d . P a b c d}) = (\<Union> (a,b,c,d) \<in> {(a,b,c,d) | a b c d . P a b c d} . f a b c d)" 
+      by blast
 
     have *: "T3 = (\<Union> (p,pt,q,A) \<in> {(p, pt, q, A) | p pt q A . \<exists>P q' t1 t2. (q, P) \<in> prs \<and> path P (FSM.initial P) p \<and> target (FSM.initial P) p = q \<and> pt \<in> tps q \<and> q' \<in> rd_targets (q, pt) \<and> (A, t1, t2) \<in> atcs (target q pt, q')}
                        . (\<lambda>io_atc. p_io p @ p_io pt @ io_atc) ` atc_to_io_set (FSM.from_FSM M (target q pt)) A)"
@@ -1252,195 +1227,22 @@ qed
 
 
 
-
-
-
-(* TODO: name *)
-lemma test_suite_to_io_pass_maximal :
-  assumes "is_sufficient_for_reduction_testing T M m"
-  and     "is_finite_test_suite T"  
-shows "pass_io_set M' (test_suite_to_io M T) = pass_io_set_maximal M' {io' \<in> (test_suite_to_io M T) . \<not> (\<exists> io'' . io'' \<noteq> [] \<and> io'@io'' \<in> (test_suite_to_io M T))}"
-proof -
-
-  (* finiteness *)
-  have p1: "finite (test_suite_to_io M T)"
-    using test_suite_to_io_finite[OF assms] by assumption
-
-  (* prefix closure *)
-  obtain prs tps rd_targets atcs where "T = Test_Suite prs tps rd_targets atcs"
-    by (meson test_suite.exhaust)
-  then obtain RepSets where RepSets_def: "is_sufficient_for_reduction_testing_for_RepSets (Test_Suite prs tps rd_targets atcs) M m RepSets"
-    using assms(1) unfolding is_sufficient_for_reduction_testing_def by blast
-  then have "is_sufficient_for_reduction_testing (Test_Suite prs tps rd_targets atcs) M m"
-    unfolding is_sufficient_for_reduction_testing_def by blast
-  then have test_suite_language_prop: "test_suite_to_io M (Test_Suite prs tps rd_targets atcs) \<subseteq> L M"
-    using test_suite_to_io_language by blast
-
-  have p2: "\<And>io' io''. io' @ io'' \<in> test_suite_to_io M T \<Longrightarrow> io' \<in> test_suite_to_io M T"
-    unfolding \<open>T = Test_Suite prs tps rd_targets atcs\<close>
-  proof -
-    fix io' io'' assume "io' @ io'' \<in> test_suite_to_io M (Test_Suite prs tps rd_targets atcs)"
-
-    have preamble_prop : "\<And> io''' q P . (q,P) \<in> prs \<Longrightarrow> io'@io''' \<in> L P \<Longrightarrow> io' \<in> test_suite_to_io M (Test_Suite prs tps rd_targets atcs)"
-    proof -
-      fix io''' q P assume "(q,P) \<in> prs" and "io'@io''' \<in> L P" 
-      have "io' \<in> (\<Union> (q,P) \<in> prs . L P)" 
-        using \<open>(q,P) \<in> prs\<close> language_prefix[OF \<open>io'@io''' \<in> L P\<close>] by auto
-      then show "io' \<in> test_suite_to_io M (Test_Suite prs tps rd_targets atcs)" 
-        unfolding test_suite_to_io.simps by blast
-    qed
-
-    have traversal_path_prop : "\<And> io''' p pt q P . io'@io''' \<in> (\<lambda> io' . p_io p @ io') ` (set (prefixes (p_io pt))) \<Longrightarrow> (q,P) \<in> prs \<Longrightarrow> path P (initial P) p \<Longrightarrow> target (initial P) p = q \<Longrightarrow> pt \<in> tps q \<Longrightarrow> io' \<in> test_suite_to_io M (Test_Suite prs tps rd_targets atcs)"
-    proof - 
-      fix io''' p pt q P assume "io'@io''' \<in> (\<lambda> io' . p_io p @ io') ` (set (prefixes (p_io pt)))"  
-                            and "(q,P) \<in> prs" 
-                            and "path P (initial P) p" 
-                            and "target (initial P) p = q" 
-                            and "pt \<in> tps q"
-
-      obtain ioP1 where "io'@io''' = p_io p @ ioP1" and "ioP1 \<in> (set (prefixes (p_io pt)))"
-        using \<open>io'@io''' \<in> (\<lambda> io' . p_io p @ io') ` (set (prefixes (p_io pt)))\<close> by auto
-      then obtain ioP2 where "ioP1 @ ioP2 = p_io pt"
-         unfolding prefixes_set by blast
-
-
-      show "io' \<in> test_suite_to_io M (Test_Suite prs tps rd_targets atcs)"
-      proof (cases "length io' \<le> length (p_io p)")
-        case True
-        then have "io' = (take (length io') (p_io p))"
-          using \<open>io'@io''' = p_io p @ ioP1\<close>
-          by (metis (no_types, lifting) order_refl take_all take_le) 
-        then have "p_io p = io'@(drop (length io') (p_io p))"
-          by (metis (no_types, lifting) append_take_drop_id)
-        then have "io'@(drop (length io') (p_io p)) \<in> L P"
-          using language_state_containment[OF \<open>path P (initial P) p\<close>] by blast
-        then show ?thesis 
-          using preamble_prop[OF \<open>(q,P) \<in> prs\<close>] by blast
-      next
-        case False
-        then have "io' = p_io p @ (take (length io' - length (p_io p)) ioP1)"
-          using \<open>io'@io''' = p_io p @ ioP1\<close>
-          by (metis (no_types, lifting) le_cases take_all take_append take_le) 
-        moreover have "(take (length io' - length (p_io p)) ioP1) \<in> (set (prefixes (p_io pt)))"
-        proof -
-          have "ioP1 = (take (length io' - length (p_io p)) ioP1) @ (drop (length io' - length (p_io p)) ioP1)"
-            by auto
-          then have "(take (length io' - length (p_io p)) ioP1) @ ((drop (length io' - length (p_io p)) ioP1) @ ioP2) = p_io pt"
-            using \<open>ioP1 @ ioP2 = p_io pt\<close> by (metis (mono_tags, lifting) append_assoc) 
-          then show ?thesis
-            unfolding prefixes_set by blast
-        qed
-        ultimately have "io' \<in> (\<lambda> io' . p_io p @ io') ` (set (prefixes (p_io pt)))"
-          by blast
-        then have "io' \<in> (\<Union>{(\<lambda> io' . p_io p @ io') ` (set (prefixes (p_io pt))) | p pt . \<exists> q P . (q,P) \<in> prs \<and> path P (initial P) p \<and> target (initial P) p = q \<and> pt \<in> tps q})"
-          using \<open>(q,P) \<in> prs\<close> \<open>path P (initial P) p\<close> \<open>target (initial P) p = q\<close> \<open>pt \<in> tps q\<close> by blast
-        then show ?thesis 
-          unfolding test_suite_to_io.simps by blast          
-      qed
-    qed
-
-
-
-    from \<open>io' @ io'' \<in> test_suite_to_io M (Test_Suite prs tps rd_targets atcs)\<close> consider
-      (a) "io' @ io'' \<in> (\<Union> (q,P) \<in> prs . L P)" |
-      (b) "io' @ io'' \<in> (\<Union>{(\<lambda> io' . p_io p @ io') ` (set (prefixes (p_io pt))) | p pt . \<exists> q P . (q,P) \<in> prs \<and> path P (initial P) p \<and> target (initial P) p = q \<and> pt \<in> tps q})" |
-      (c) "io' @ io'' \<in> (\<Union>{(\<lambda> io_atc . p_io p @ p_io pt @ io_atc) ` (atc_to_io_set (from_FSM M (target q pt)) A) | p pt q A . \<exists> P q' t1 t2 . (q,P) \<in> prs \<and> path P (initial P) p \<and> target (initial P) p = q \<and> pt \<in> tps q \<and> q' \<in> rd_targets (q,pt) \<and> (A,t1,t2) \<in> atcs (target q pt,q') })"
-      unfolding test_suite_to_io.simps
-      by blast
-
-    then show "io' \<in> test_suite_to_io M (Test_Suite prs tps rd_targets atcs)" 
-    proof cases
-      case a
-      then show ?thesis using preamble_prop by blast
-    next
-      case b
-      then show ?thesis using traversal_path_prop by blast
-    next
-      case c
-      then obtain p pt q A  P q' t1 t2  where "io' @ io'' \<in> (\<lambda> io_atc . p_io p @ p_io pt @ io_atc) ` (atc_to_io_set (from_FSM M (target q pt)) A)"
-                                          and "(q,P) \<in> prs" 
-                                          and "path P (initial P) p"
-                                          and "target (initial P) p = q"
-                                          and "pt \<in> tps q"
-                                          and "q' \<in> rd_targets (q,pt)"
-                                          and "(A,t1,t2) \<in> atcs (target q pt,q')"
-        by blast
-
-      obtain ioA where "io' @ io'' = p_io p @ p_io pt @ ioA" 
-                   and "ioA \<in> (atc_to_io_set (from_FSM M (target q pt)) A)"
-        using \<open>io' @ io'' \<in> (\<lambda> io_atc . p_io p @ p_io pt @ io_atc) ` (atc_to_io_set (from_FSM M (target q pt)) A)\<close> 
-        by blast
-
-      
-
-      show ?thesis proof (cases "length io' \<le> length (p_io p @ p_io pt)")
-        case True
-        then have "io' @ (drop (length io') (p_io p @ p_io pt)) = p_io p @ p_io pt"
-          using \<open>io' @ io'' = p_io p @ p_io pt @ ioA\<close>
-          by (simp add: append_eq_conv_conj) 
-        moreover have "p_io p @ p_io pt \<in> (\<lambda> io' . p_io p @ io') ` (set (prefixes (p_io pt)))"
-          unfolding prefixes_set by blast
-        ultimately have "io'@(drop (length io') (p_io p @ p_io pt)) \<in> (\<lambda> io' . p_io p @ io') ` (set (prefixes (p_io pt)))"
-          by simp
-        then show ?thesis 
-          using traversal_path_prop[OF _ \<open>(q,P) \<in> prs\<close> \<open>path P (initial P) p\<close> \<open>target (initial P) p = q\<close> \<open>pt \<in> tps q\<close>] by blast
-      next
-        case False
-        then have "io' = (p_io p @ p_io pt) @ (take (length io' - length (p_io p @ p_io pt)) ioA)"
-        proof -
-          have "io' = take (length io') (io' @ io'')"
-            by auto
-          then show ?thesis
-            using False \<open>io' @ io'' = p_io p @ p_io pt @ ioA\<close> by fastforce
-        qed
-        moreover have "(take (length io' - length (p_io p @ p_io pt)) ioA) \<in> (atc_to_io_set (from_FSM M (target q pt)) A)"
-        proof -
-          have "(take (length io' - length (p_io p @ p_io pt)) ioA)@(drop (length io' - length (p_io p @ p_io pt)) ioA) \<in> L (from_FSM M (target q pt)) \<inter> L A"
-            using \<open>ioA \<in> (atc_to_io_set (from_FSM M (target q pt)) A)\<close> by auto
-          then have *: "(take (length io' - length (p_io p @ p_io pt)) ioA)@(drop (length io' - length (p_io p @ p_io pt)) ioA) \<in> L (from_FSM M (target q pt))"
-               and **: "(take (length io' - length (p_io p @ p_io pt)) ioA)@(drop (length io' - length (p_io p @ p_io pt)) ioA) \<in> L A"
-            by blast+
-          show ?thesis
-            using language_prefix[OF *] language_prefix[OF **]
-            unfolding atc_to_io_set.simps by blast
-        qed
-        ultimately have "io' \<in> (\<lambda> io_atc . p_io p @ p_io pt @ io_atc) ` (atc_to_io_set (from_FSM M (target q pt)) A)"
-          by force
-            
-        then have "io' \<in> (\<Union>{(\<lambda> io_atc . p_io p @ p_io pt @ io_atc) ` (atc_to_io_set (from_FSM M (target q pt)) A) | p pt q A . \<exists> P q' t1 t2 . (q,P) \<in> prs \<and> path P (initial P) p \<and> target (initial P) p = q \<and> pt \<in> tps q \<and> q' \<in> rd_targets (q,pt) \<and> (A,t1,t2) \<in> atcs (target q pt,q') })"
-          using \<open>(q,P) \<in> prs\<close> \<open>path P (initial P) p\<close> \<open>target (initial P) p = q\<close> \<open>pt \<in> tps q\<close> \<open>q' \<in> rd_targets (q,pt)\<close> \<open>(A,t1,t2) \<in> atcs (target q pt,q')\<close> by blast
-        then show ?thesis 
-          unfolding test_suite_to_io.simps by blast
-      qed
-    qed
-  qed
-
-
-  then show ?thesis
-    using pass_io_set_maximal_from_pass_io_set[OF p1] by blast
-qed
-
-
-
-
-
-
-
 subsection \<open>Calculating the Sets of Sequences\<close>
-
-
 
 
 abbreviation "L_acyclic M \<equiv> LS_acyclic M (initial M)"
 
 (* collect the prefix-closed IO-sequence representation of a test suite for some reference FSM *)
 fun test_suite_to_io' :: "('a,'b,'c) fsm \<Rightarrow> ('a,'b,'c,'d) test_suite \<Rightarrow> ('b \<times> 'c) list set" where
-  "test_suite_to_io' M (Test_Suite prs tps rd_targets atcs) = (\<Union> (q,P) \<in> prs . L_acyclic P \<union> (\<Union> ioP \<in> remove_proper_prefixes (L_acyclic P) . \<Union> pt \<in> tps q . ((\<lambda> io' . ioP @ io') ` (set (prefixes (p_io pt)))) \<union> (\<Union> q' \<in> rd_targets (q,pt) . \<Union> (A,t1,t2) \<in> atcs (target q pt,q') . (\<lambda> io_atc . ioP @ p_io pt @ io_atc) ` (acyclic_language_intersection (from_FSM M (target q pt)) A))))"
-
-(* slightly optimized calculation of the test suite representation using only maximal IO-sequences *)
-fun test_suite_to_io'_maximal :: "('a::linorder,'b::linorder,'c::linorder) fsm \<Rightarrow> ('a,'b,'c,'d::linorder) test_suite \<Rightarrow> ('b \<times> 'c) list set" where
-  "test_suite_to_io'_maximal M (Test_Suite prs tps rd_targets atcs) = 
-      remove_proper_prefixes (\<Union> (q,P) \<in> prs . L_acyclic P \<union> (\<Union> ioP \<in> remove_proper_prefixes (L_acyclic P) . \<Union> pt \<in> tps q . Set.insert (ioP @ p_io pt) (\<Union> q' \<in> rd_targets (q,pt) . \<Union> (A,t1,t2) \<in> atcs (target q pt,q') . (\<lambda> io_atc . ioP @ p_io pt @ io_atc) ` (remove_proper_prefixes (acyclic_language_intersection (from_FSM M (target q pt)) A)))))"
+  "test_suite_to_io' M (Test_Suite prs tps rd_targets atcs) 
+      = (\<Union> (q,P) \<in> prs . 
+          L_acyclic P 
+          \<union> (\<Union> ioP \<in> remove_proper_prefixes (L_acyclic P) . 
+              \<Union> pt \<in> tps q . 
+                ((\<lambda> io' . ioP @ io') ` (set (prefixes (p_io pt)))) 
+                \<union> (\<Union> q' \<in> rd_targets (q,pt) . 
+                    \<Union> (A,t1,t2) \<in> atcs (target q pt,q') . 
+                      (\<lambda> io_atc . ioP @ p_io pt @ io_atc) ` (acyclic_language_intersection (from_FSM M (target q pt)) A))))"
 
 
 lemma test_suite_to_io_code :
@@ -1453,25 +1255,25 @@ proof -
   obtain prs tps rd_targets atcs where "T = Test_Suite prs tps rd_targets atcs"
     by (meson test_suite.exhaust)
 
-
-
   then obtain RepSets where RepSets_def: "is_sufficient_for_reduction_testing_for_RepSets (Test_Suite prs tps rd_targets atcs) M m RepSets"
-    using assms(1) unfolding is_sufficient_for_reduction_testing_def by blast
-
-
+    using assms(1) 
+    unfolding is_sufficient_for_reduction_testing_def 
+    by blast
 
   have t2: "\<And> q P. (q, P) \<in> prs \<Longrightarrow> is_preamble P M q"
-    using is_sufficient_for_reduction_testing_for_RepSets_simps(2)[OF RepSets_def] by blast
+    using is_sufficient_for_reduction_testing_for_RepSets_simps(2)[OF RepSets_def] 
+    by blast
   have t3: "\<And> q1 q2 A d1 d2. (A, d1, d2) \<in> atcs (q1, q2) \<Longrightarrow> (A, d2, d1) \<in> atcs (q2, q1) \<and> is_separator M q1 q2 A d1 d2"
-    using is_sufficient_for_reduction_testing_for_RepSets_simps(3)[OF RepSets_def] by assumption
+    using is_sufficient_for_reduction_testing_for_RepSets_simps(3)[OF RepSets_def] 
+    by assumption
 
 
-
-  have test_suite_to_io'_alt_def: "test_suite_to_io' M T  = (\<Union> (q,P) \<in> prs . L_acyclic P)
-    \<union> (\<Union> (q,P) \<in> prs . \<Union> ioP \<in> remove_proper_prefixes (L_acyclic P) . \<Union> pt \<in> tps q . ((\<lambda> io' . ioP @ io') ` (set (prefixes (p_io pt))))) 
-    \<union> (\<Union> (q,P) \<in> prs . \<Union> ioP \<in> remove_proper_prefixes (L_acyclic P) . \<Union> pt \<in> tps q . \<Union> q' \<in> rd_targets (q,pt) . \<Union> (A,t1,t2) \<in> atcs (target q pt,q') . (\<lambda> io_atc . ioP @ p_io pt @ io_atc) ` (acyclic_language_intersection (from_FSM M (target q pt)) A))"
+  have test_suite_to_io'_alt_def: "test_suite_to_io' M T  
+    = (\<Union> (q,P) \<in> prs . L_acyclic P)
+      \<union> (\<Union> (q,P) \<in> prs . \<Union> ioP \<in> remove_proper_prefixes (L_acyclic P) . \<Union> pt \<in> tps q . ((\<lambda> io' . ioP @ io') ` (set (prefixes (p_io pt))))) 
+      \<union> (\<Union> (q,P) \<in> prs . \<Union> ioP \<in> remove_proper_prefixes (L_acyclic P) . \<Union> pt \<in> tps q . \<Union> q' \<in> rd_targets (q,pt) . \<Union> (A,t1,t2) \<in> atcs (target q pt,q') . (\<lambda> io_atc . ioP @ p_io pt @ io_atc) ` (acyclic_language_intersection (from_FSM M (target q pt)) A))"
     unfolding test_suite_to_io'.simps \<open>T = Test_Suite prs tps rd_targets atcs\<close> 
-    by force
+    by fast
 
   have test_suite_to_io_alt_def: "test_suite_to_io M T =
     (\<Union> (q,P) \<in> prs . L P)
@@ -1622,6 +1424,19 @@ qed
 
 
 
+
+
+
+
+subsection \<open>Using Maximal Sequences Only\<close>
+
+
+
+fun test_suite_to_io'_maximal :: "('a::linorder,'b::linorder,'c::linorder) fsm \<Rightarrow> ('a,'b,'c,'d::linorder) test_suite \<Rightarrow> ('b \<times> 'c) list set" where
+  "test_suite_to_io'_maximal M (Test_Suite prs tps rd_targets atcs) = 
+      remove_proper_prefixes (\<Union> (q,P) \<in> prs . L_acyclic P \<union> (\<Union> ioP \<in> remove_proper_prefixes (L_acyclic P) . \<Union> pt \<in> tps q . Set.insert (ioP @ p_io pt) (\<Union> q' \<in> rd_targets (q,pt) . \<Union> (A,t1,t2) \<in> atcs (target q pt,q') . (\<lambda> io_atc . ioP @ p_io pt @ io_atc) ` (remove_proper_prefixes (acyclic_language_intersection (from_FSM M (target q pt)) A)))))"
+
+
 lemma test_suite_to_io'_maximal_code : 
   assumes "is_sufficient_for_reduction_testing T M m"
   and     "is_finite_test_suite T"  
@@ -1631,7 +1446,6 @@ proof -
 
   obtain prs tps rd_targets atcs where "T = Test_Suite prs tps rd_targets atcs"
     by (meson test_suite.exhaust)
-
 
   have t_def: "test_suite_to_io M T = test_suite_to_io' M T"
     using test_suite_to_io_code[OF assms] by assumption
@@ -1806,8 +1620,167 @@ proof -
 qed
 
 
+lemma test_suite_to_io_pass_maximal :
+  assumes "is_sufficient_for_reduction_testing T M m"
+  and     "is_finite_test_suite T"  
+shows "pass_io_set M' (test_suite_to_io M T) = pass_io_set_maximal M' {io' \<in> (test_suite_to_io M T) . \<not> (\<exists> io'' . io'' \<noteq> [] \<and> io'@io'' \<in> (test_suite_to_io M T))}"
+proof -
+
+  (* finiteness *)
+  have p1: "finite (test_suite_to_io M T)"
+    using test_suite_to_io_finite[OF assms] by assumption
+
+  (* prefix closure *)
+  obtain prs tps rd_targets atcs where "T = Test_Suite prs tps rd_targets atcs"
+    by (meson test_suite.exhaust)
+  then obtain RepSets where RepSets_def: "is_sufficient_for_reduction_testing_for_RepSets (Test_Suite prs tps rd_targets atcs) M m RepSets"
+    using assms(1) unfolding is_sufficient_for_reduction_testing_def by blast
+  then have "is_sufficient_for_reduction_testing (Test_Suite prs tps rd_targets atcs) M m"
+    unfolding is_sufficient_for_reduction_testing_def by blast
+  then have test_suite_language_prop: "test_suite_to_io M (Test_Suite prs tps rd_targets atcs) \<subseteq> L M"
+    using test_suite_to_io_language by blast
+
+  have p2: "\<And>io' io''. io' @ io'' \<in> test_suite_to_io M T \<Longrightarrow> io' \<in> test_suite_to_io M T"
+    unfolding \<open>T = Test_Suite prs tps rd_targets atcs\<close>
+  proof -
+    fix io' io'' assume "io' @ io'' \<in> test_suite_to_io M (Test_Suite prs tps rd_targets atcs)"
+
+    have preamble_prop : "\<And> io''' q P . (q,P) \<in> prs \<Longrightarrow> io'@io''' \<in> L P \<Longrightarrow> io' \<in> test_suite_to_io M (Test_Suite prs tps rd_targets atcs)"
+    proof -
+      fix io''' q P assume "(q,P) \<in> prs" and "io'@io''' \<in> L P" 
+      have "io' \<in> (\<Union> (q,P) \<in> prs . L P)" 
+        using \<open>(q,P) \<in> prs\<close> language_prefix[OF \<open>io'@io''' \<in> L P\<close>] by auto
+      then show "io' \<in> test_suite_to_io M (Test_Suite prs tps rd_targets atcs)" 
+        unfolding test_suite_to_io.simps by blast
+    qed
+
+    have traversal_path_prop : "\<And> io''' p pt q P . io'@io''' \<in> (\<lambda> io' . p_io p @ io') ` (set (prefixes (p_io pt))) \<Longrightarrow> (q,P) \<in> prs \<Longrightarrow> path P (initial P) p \<Longrightarrow> target (initial P) p = q \<Longrightarrow> pt \<in> tps q \<Longrightarrow> io' \<in> test_suite_to_io M (Test_Suite prs tps rd_targets atcs)"
+    proof - 
+      fix io''' p pt q P assume "io'@io''' \<in> (\<lambda> io' . p_io p @ io') ` (set (prefixes (p_io pt)))"  
+                            and "(q,P) \<in> prs" 
+                            and "path P (initial P) p" 
+                            and "target (initial P) p = q" 
+                            and "pt \<in> tps q"
+
+      obtain ioP1 where "io'@io''' = p_io p @ ioP1" and "ioP1 \<in> (set (prefixes (p_io pt)))"
+        using \<open>io'@io''' \<in> (\<lambda> io' . p_io p @ io') ` (set (prefixes (p_io pt)))\<close> by auto
+      then obtain ioP2 where "ioP1 @ ioP2 = p_io pt"
+         unfolding prefixes_set by blast
 
 
+      show "io' \<in> test_suite_to_io M (Test_Suite prs tps rd_targets atcs)"
+      proof (cases "length io' \<le> length (p_io p)")
+        case True
+        then have "io' = (take (length io') (p_io p))"
+          using \<open>io'@io''' = p_io p @ ioP1\<close>
+          by (metis (no_types, lifting) order_refl take_all take_le) 
+        then have "p_io p = io'@(drop (length io') (p_io p))"
+          by (metis (no_types, lifting) append_take_drop_id)
+        then have "io'@(drop (length io') (p_io p)) \<in> L P"
+          using language_state_containment[OF \<open>path P (initial P) p\<close>] by blast
+        then show ?thesis 
+          using preamble_prop[OF \<open>(q,P) \<in> prs\<close>] by blast
+      next
+        case False
+        then have "io' = p_io p @ (take (length io' - length (p_io p)) ioP1)"
+          using \<open>io'@io''' = p_io p @ ioP1\<close>
+          by (metis (no_types, lifting) le_cases take_all take_append take_le) 
+        moreover have "(take (length io' - length (p_io p)) ioP1) \<in> (set (prefixes (p_io pt)))"
+        proof -
+          have "ioP1 = (take (length io' - length (p_io p)) ioP1) @ (drop (length io' - length (p_io p)) ioP1)"
+            by auto
+          then have "(take (length io' - length (p_io p)) ioP1) @ ((drop (length io' - length (p_io p)) ioP1) @ ioP2) = p_io pt"
+            using \<open>ioP1 @ ioP2 = p_io pt\<close> by (metis (mono_tags, lifting) append_assoc) 
+          then show ?thesis
+            unfolding prefixes_set by blast
+        qed
+        ultimately have "io' \<in> (\<lambda> io' . p_io p @ io') ` (set (prefixes (p_io pt)))"
+          by blast
+        then have "io' \<in> (\<Union>{(\<lambda> io' . p_io p @ io') ` (set (prefixes (p_io pt))) | p pt . \<exists> q P . (q,P) \<in> prs \<and> path P (initial P) p \<and> target (initial P) p = q \<and> pt \<in> tps q})"
+          using \<open>(q,P) \<in> prs\<close> \<open>path P (initial P) p\<close> \<open>target (initial P) p = q\<close> \<open>pt \<in> tps q\<close> by blast
+        then show ?thesis 
+          unfolding test_suite_to_io.simps by blast          
+      qed
+    qed
+
+
+    from \<open>io' @ io'' \<in> test_suite_to_io M (Test_Suite prs tps rd_targets atcs)\<close> consider
+      (a) "io' @ io'' \<in> (\<Union> (q,P) \<in> prs . L P)" |
+      (b) "io' @ io'' \<in> (\<Union>{(\<lambda> io' . p_io p @ io') ` (set (prefixes (p_io pt))) | p pt . \<exists> q P . (q,P) \<in> prs \<and> path P (initial P) p \<and> target (initial P) p = q \<and> pt \<in> tps q})" |
+      (c) "io' @ io'' \<in> (\<Union>{(\<lambda> io_atc . p_io p @ p_io pt @ io_atc) ` (atc_to_io_set (from_FSM M (target q pt)) A) | p pt q A . \<exists> P q' t1 t2 . (q,P) \<in> prs \<and> path P (initial P) p \<and> target (initial P) p = q \<and> pt \<in> tps q \<and> q' \<in> rd_targets (q,pt) \<and> (A,t1,t2) \<in> atcs (target q pt,q') })"
+      unfolding test_suite_to_io.simps
+      by blast
+
+    then show "io' \<in> test_suite_to_io M (Test_Suite prs tps rd_targets atcs)" 
+    proof cases
+      case a
+      then show ?thesis using preamble_prop by blast
+    next
+      case b
+      then show ?thesis using traversal_path_prop by blast
+    next
+      case c
+      then obtain p pt q A  P q' t1 t2  where "io' @ io'' \<in> (\<lambda> io_atc . p_io p @ p_io pt @ io_atc) ` (atc_to_io_set (from_FSM M (target q pt)) A)"
+                                          and "(q,P) \<in> prs" 
+                                          and "path P (initial P) p"
+                                          and "target (initial P) p = q"
+                                          and "pt \<in> tps q"
+                                          and "q' \<in> rd_targets (q,pt)"
+                                          and "(A,t1,t2) \<in> atcs (target q pt,q')"
+        by blast
+
+      obtain ioA where "io' @ io'' = p_io p @ p_io pt @ ioA" 
+                   and "ioA \<in> (atc_to_io_set (from_FSM M (target q pt)) A)"
+        using \<open>io' @ io'' \<in> (\<lambda> io_atc . p_io p @ p_io pt @ io_atc) ` (atc_to_io_set (from_FSM M (target q pt)) A)\<close> 
+        by blast
+
+
+      show ?thesis proof (cases "length io' \<le> length (p_io p @ p_io pt)")
+        case True
+        then have "io' @ (drop (length io') (p_io p @ p_io pt)) = p_io p @ p_io pt"
+          using \<open>io' @ io'' = p_io p @ p_io pt @ ioA\<close>
+          by (simp add: append_eq_conv_conj) 
+        moreover have "p_io p @ p_io pt \<in> (\<lambda> io' . p_io p @ io') ` (set (prefixes (p_io pt)))"
+          unfolding prefixes_set by blast
+        ultimately have "io'@(drop (length io') (p_io p @ p_io pt)) \<in> (\<lambda> io' . p_io p @ io') ` (set (prefixes (p_io pt)))"
+          by simp
+        then show ?thesis 
+          using traversal_path_prop[OF _ \<open>(q,P) \<in> prs\<close> \<open>path P (initial P) p\<close> \<open>target (initial P) p = q\<close> \<open>pt \<in> tps q\<close>] by blast
+      next
+        case False
+        then have "io' = (p_io p @ p_io pt) @ (take (length io' - length (p_io p @ p_io pt)) ioA)"
+        proof -
+          have "io' = take (length io') (io' @ io'')"
+            by auto
+          then show ?thesis
+            using False \<open>io' @ io'' = p_io p @ p_io pt @ ioA\<close> by fastforce
+        qed
+        moreover have "(take (length io' - length (p_io p @ p_io pt)) ioA) \<in> (atc_to_io_set (from_FSM M (target q pt)) A)"
+        proof -
+          have "(take (length io' - length (p_io p @ p_io pt)) ioA)@(drop (length io' - length (p_io p @ p_io pt)) ioA) \<in> L (from_FSM M (target q pt)) \<inter> L A"
+            using \<open>ioA \<in> (atc_to_io_set (from_FSM M (target q pt)) A)\<close> by auto
+          then have *: "(take (length io' - length (p_io p @ p_io pt)) ioA)@(drop (length io' - length (p_io p @ p_io pt)) ioA) \<in> L (from_FSM M (target q pt))"
+               and **: "(take (length io' - length (p_io p @ p_io pt)) ioA)@(drop (length io' - length (p_io p @ p_io pt)) ioA) \<in> L A"
+            by blast+
+          show ?thesis
+            using language_prefix[OF *] language_prefix[OF **]
+            unfolding atc_to_io_set.simps by blast
+        qed
+        ultimately have "io' \<in> (\<lambda> io_atc . p_io p @ p_io pt @ io_atc) ` (atc_to_io_set (from_FSM M (target q pt)) A)"
+          by force
+            
+        then have "io' \<in> (\<Union>{(\<lambda> io_atc . p_io p @ p_io pt @ io_atc) ` (atc_to_io_set (from_FSM M (target q pt)) A) | p pt q A . \<exists> P q' t1 t2 . (q,P) \<in> prs \<and> path P (initial P) p \<and> target (initial P) p = q \<and> pt \<in> tps q \<and> q' \<in> rd_targets (q,pt) \<and> (A,t1,t2) \<in> atcs (target q pt,q') })"
+          using \<open>(q,P) \<in> prs\<close> \<open>path P (initial P) p\<close> \<open>target (initial P) p = q\<close> \<open>pt \<in> tps q\<close> \<open>q' \<in> rd_targets (q,pt)\<close> \<open>(A,t1,t2) \<in> atcs (target q pt,q')\<close> by blast
+        then show ?thesis 
+          unfolding test_suite_to_io.simps by blast
+      qed
+    qed
+  qed
+
+
+  then show ?thesis
+    using pass_io_set_maximal_from_pass_io_set[OF p1] by blast
+qed
 
 
 
@@ -1827,9 +1800,6 @@ shows     "(L M' \<subseteq> L M) \<longleftrightarrow> pass_io_set_maximal M' (
   unfolding test_suite_to_io_pass_maximal[OF assms(1,2)]
   unfolding test_suite_to_io'_maximal_code[OF assms(1,2,3)]
   by simp
-
-
-
 
 
 end
